@prefix : <http://pid.geoscience.org.au/def/ont/link#> .
@prefix owl: <http://www.w3.org/2002/07/owl#> .
@prefix rdf: <http://www.w3.org/1999/02/22-rdf-syntax-ns#> .
@prefix reg: <http://purl.org/linked-data/registry#> .
@prefix xml: <http://www.w3.org/XML/1998/namespace> .
@prefix xsd: <http://www.w3.org/2001/XMLSchema#> .
@prefix dcat: <http://www.w3.org/ns/dcat#> .
@prefix rdfs: <http://www.w3.org/2000/01/rdf-schema#> .
@prefix sosa: <http://www.w3.org/ns/sosa/> .
@prefix vann: <http://purl.org/vocab/vann/> .
@prefix dcterms: <http://purl.org/dc/terms/> .
@base <http://pid.geoscience.org.au/def/ont/link#> .

<http://pid.geoscience.org.au/def/ont/link#> rdf:type owl:Ontology ;
                                              owl:versionIRI <http://pid.geoscience.org.au/def/ont/link/1.0> ;
                                              owl:imports <http://www.w3.org/ns/dcat> ,
                                                          <http://purl.org/linked-data/registry> ,
                                                          <http://promsns.org/def/agr/1.1> ,
                                                          <http://www.w3.org/ns/prov> ,
                                                          <http://www.w3.org/ns/org#> ;
                                              owl:versionInfo 1.1 ;
                                              dcterms:description """An OWL ontology for all the information within the [LINK System](http://link.fsdf.org.au) which itself is within the Foundational Spatial Data Framework (FSDF) initative.

This ontology contains classes for all of the major information objects that the LINK system publishes. The LINK system uses a web Content Management System to manage the data which has its own database. In order for that information to be interoperable with information in other applications, the LINK information is mapped to a series of 'upper' (generic) ontologies (data models) which information in other applications can then also be mapped to. So an 'Agency' in the LINK is mapped to an [ORG](https://www.w3.org/TR/vocab-org/) ontology 'Organisation' so other information understanding an Organisation will understand something about a LINK Agency."""@en ;
                                              rdfs:seeAlso <https://github.com/nicholascar/link-o> ;
                                              dcterms:creator "Nicholas Car"@en ;
                                              dcterms:title "LINK Ontology"@en ;
                                              rdfs:comment """An OWL ontology for all the information within the [LINK System](http://link.fsdf.org.au) which itself is within the Foundational Spatial Data Framework (FSDF) initative.

This ontology contains classes for all of the major information objects that the LINK system publishes. The LINK system uses a web Content Management System to manage the data which has its own database. In order for that information to be interoperable with information in other applications, the LINK information is mapped to a series of 'upper' (generic) ontologies (data models) which information in other applications can then also be mapped to. So an 'Agency' in the LINK is mapped to an [ORG](https://www.w3.org/TR/vocab-org/) ontology 'Organisation' so other information understanding an Organisation will understand something about a LINK Agency."""@en ;
                                              dcterms:license <https://creativecommons.org/licenses/by/4.0/> ;
                                              vann:preferredNamespaceUri "http://pid.geoscience.org.au/def/ont/link#"@en ;
                                              dcterms:creator <http://orcid.org/0000-0002-8742-7730> ;
                                              dcterms:created "2016-12-08"^^xsd:date ;
                                              vann:preferredNamespacePrefix "link"@en ;
                                              rdfs:isDefinedBy <http://pid.geoscience.org.au/def/ont/link> ;
                                              dcterms:modified "2017-06-14"@en ;
                                              dcterms:rights "(c) Geoscience Australia 2017"@en ;
                                              rdfs:label "LINK ontology"@en .

#################################################################
#    Annotation properties
#################################################################

###  http://purl.org/linked-data/registry#containedItemClass
reg:containedItemClass rdf:type owl:AnnotationProperty .


###  http://purl.org/linked-data/registry#subregister
reg:subregister rdf:type owl:AnnotationProperty .


#################################################################
#    Object Properties
#################################################################

###  http://pid.geoscience.org.au/def/ont/link#hasJurisdiction
:hasJurisdiction rdf:type owl:ObjectProperty ;
                 rdfs:subPropertyOf <http://www.w3.org/ns/org#subOrganizationOf> ;
                 owl:inverseOf :jurisdictionOf ;
                 rdfs:domain <http://www.w3.org/ns/prov#Entity> ;
                 rdfs:range :Jurisdiction ;
                 rdfs:comment "A Dataset may have a hasJuristiction property indicating its Jurisdiction" ;
                 rdfs:label "has jurisdiction" .


###  http://pid.geoscience.org.au/def/ont/link#jurisdictionOf
:jurisdictionOf rdf:type owl:ObjectProperty ;
                rdfs:subPropertyOf <http://www.w3.org/ns/org#hasSubOrganization> ;
                rdfs:comment "Inverse of hasJurisdiction" ;
                rdfs:label "jurisdiction of" .


###  http://pid.geoscience.org.au/def/ont/link#wasMandatedBy
:wasMandatedBy rdf:type owl:ObjectProperty ;
               rdfs:subPropertyOf <http://www.w3.org/ns/prov#wasInfluencedBy> ;
               rdfs:domain <http://www.w3.org/ns/prov#Entity> ;
               rdfs:range :Mandate ;
               rdfs:label """The production of a Dataset wasMandatedBy a particular Mandate. 

This is equivalent to a Dataset (prov:Entity) being influence by (prov:wasInfluencedBy) a Mandate (prov:Entity) where the influence is qualified by using a prov:qualifiedInfluence indicating a prov:Influence which in turn indicates the Mandate (via prov:entity) and a role that the Mandate tool (via prov:role) which can be assumed to be something like \"Mandate\" which is left undefined at this point.""" ,
                          "was mandated by" .


#################################################################
#    Classes
#################################################################

###  http://pid.geoscience.org.au/def/ont/link#Agency
:Agency rdf:type owl:Class ;
        rdfs:subClassOf <http://www.w3.org/ns/prov#Organization> ;
        rdfs:comment "An Agency is any government organisation that produces or publishes Datasets"@en ;
        rdfs:label "Agency"@en .


###  http://pid.geoscience.org.au/def/ont/link#Dataset
:Dataset rdf:type owl:Class ;
         rdfs:subClassOf dcat:Dataset ,
                         <http://www.w3.org/ns/prov#Entity> ;
         rdfs:comment "LINK's Datasets are both DCAT Datasets and also PROV Entities. This means they can have metadata according to DCAT and relations to other Datasets, Agents and Activities according to PROV."@en ;
         rdfs:label "Dataset"@en .


###  http://pid.geoscience.org.au/def/ont/link#FSDFDatasetCollection
:FSDFDatasetCollection rdf:type owl:Class ;
                       rdfs:subClassOf <http://www.w3.org/ns/prov#Collection> ;
                       rdfs:comment "An FSDFDatasetCollection is a collection of Output Datasets generated by an FSDF Agency and categorised with an FSDFTheme. FDSFDatasetCollections are identified in the FSDF initiative's agreement."^^xsd:string ;
                       rdfs:label "FSDF Dataset Collection"^^xsd:string .


###  http://pid.geoscience.org.au/def/ont/link#FSDFTheme
:FSDFTheme rdf:type owl:Class ;
           rdfs:subClassOf <http://www.w3.org/2004/02/skos/core#Concept> ;
           rdfs:comment "An FSDFTheme is a category of Datasets (and perhaps later Activities also), used by the FSDF initiative."@en ;
           rdfs:label "FSDF Theme"@en .


###  http://pid.geoscience.org.au/def/ont/link#InputDataset
:InputDataset rdf:type owl:Class ;
              rdfs:subClassOf :Dataset ;
              rdfs:comment "An InputDataset is a Dataset published by an Agency that is an input to a process resulting in the generation of a NationalDataset."^^xsd:string ;
              rdfs:label "Input Dataset"^^xsd:string .


###  http://pid.geoscience.org.au/def/ont/link#Jurisdiction
:Jurisdiction rdf:type owl:Class ;
              rdfs:subClassOf <http://www.w3.org/2004/02/skos/core#Concept> ,
                              <http://www.w3.org/ns/org#Organization> ;
              rdfs:comment "A Jurisdiction is a State or Federal government, e.g. NSW Government"^^xsd:string ;
              rdfs:label "Jurisdiction"^^xsd:string .


###  http://pid.geoscience.org.au/def/ont/link#Mandate
:Mandate rdf:type owl:Class ;
         rdfs:subClassOf <http://promsns.org/def/agr#Agreement> ;
         rdfs:comment "A Mandate is an Act of a parliament or a governmental or Agency policy that motivates the production of Datasets."^^xsd:string ;
         rdfs:label "Mandate"^^xsd:string .


###  http://pid.geoscience.org.au/def/ont/link#NationalDataset
:NationalDataset rdf:type owl:Class ;
                 rdfs:subClassOf :Dataset ;
                 rdfs:comment "A NationalDataset is a Dataset of national significance, a Master Dataset in some terminology, thich is generated by processing of InputDatasets and from which FSDFDatasets are produced."^^xsd:string ;
                 rdfs:label "National Dataset"^^xsd:string .


###  http://pid.geoscience.org.au/def/ont/link#OutputDataset
:OutputDataset rdf:type owl:Class ;
               rdfs:subClassOf :Dataset ;
               rdfs:comment "An Output Dataset is an output of an FSDF process"^^xsd:string ;
               rdfs:label "Output Dataset"^^xsd:string .


#################################################################
#    Individuals
#################################################################

###  http://link.fsdf.org.au/dataset/
<http://link.fsdf.org.au/dataset/> rdf:type owl:NamedIndividual ,
                                            reg:Register ;
                                   reg:containedItemClass :Dataset ;
                                   rdfs:comment "The Datasets register within the LINK Content Management System"@en ;
                                   rdfs:label "eCat Dataset Register"@en .


###  http://pid.geoscience.gov.au/dataset/
<http://pid.geoscience.gov.au/dataset/> rdf:type owl:NamedIndividual ,
                                                 reg:Register ;
                                        reg:containedItemClass :Dataset ;
                                        reg:subregister <http://link.fsdf.org.au/dataset/> ;
                                        rdfs:comment "Geosceicne Australia's conceptual Datasets register, of which the LINK is a federated subregister"@en ;
                                        rdfs:label "eCat Dataset Register"@en .


###  http://pid.geoscience.org.au/def/ont/link#ACT
:ACT rdf:type owl:NamedIndividual ,
              :Jurisdiction ;
     rdfs:comment "The Australian Capital Territory government"@en ;
     rdfs:label "Australian Capital Territory"^^xsd:string .


###  http://pid.geoscience.org.au/def/ont/link#AdministrativeBoundaries
:AdministrativeBoundaries rdf:type owl:NamedIndividual ,
                                   :FSDFTheme ;
                          rdfs:comment "The Administrative Boundaries FSDF Theme"@en ;
                          rdfs:label "Administrative Boundaries"^^xsd:string .


###  http://pid.geoscience.org.au/def/ont/link#Commonwealth
:Commonwealth rdf:type owl:NamedIndividual ,
                       :Jurisdiction ;
              rdfs:comment "The Commonwealth government"@en ;
              rdfs:label "Commonwealth"^^xsd:string .


###  http://pid.geoscience.org.au/def/ont/link#ElevationAndDepth
:ElevationAndDepth rdf:type owl:NamedIndividual ,
                            :FSDFTheme ;
                   rdfs:comment "The Elevation And Depth FSDF Theme"@en ;
                   rdfs:label "Elevation And Depth"^^xsd:string .


###  http://pid.geoscience.org.au/def/ont/link#GeocodedAddressing
:GeocodedAddressing rdf:type owl:NamedIndividual ,
                             :FSDFTheme ;
                    rdfs:comment "The Geocoded Addressing FSDF Theme"@en ;
                    rdfs:label "Geocoded Addressing"^^xsd:string .


###  http://pid.geoscience.org.au/def/ont/link#Imagery
:Imagery rdf:type owl:NamedIndividual ,
                  :FSDFTheme ;
         rdfs:comment "The Imagery FSDF Theme"@en ;
         rdfs:label "Imagery"^^xsd:string .


###  http://pid.geoscience.org.au/def/ont/link#LandCoverAndLandUse
:LandCoverAndLandUse rdf:type owl:NamedIndividual ,
                              :FSDFTheme ;
                     rdfs:comment "The Land Cover And Use FSDF Theme"@en ;
                     rdfs:label "Land Cover And Use"^^xsd:string .


###  http://pid.geoscience.org.au/def/ont/link#LandParcelAndProperty
:LandParcelAndProperty rdf:type owl:NamedIndividual ,
                                :FSDFTheme ;
                       rdfs:comment "The Land Parcel and Property FSDF Theme"@en ;
                       rdfs:label "Land Parcel and Property"^^xsd:string .


###  http://pid.geoscience.org.au/def/ont/link#NSW
:NSW rdf:type owl:NamedIndividual ,
              :Jurisdiction ;
     rdfs:comment "The New South Wales state government"@en ;
     rdfs:label "New South Wales"^^xsd:string .


###  http://pid.geoscience.org.au/def/ont/link#NT
:NT rdf:type owl:NamedIndividual ,
             :Jurisdiction ;
    rdfs:comment "The Northern Territory government"@en ;
    rdfs:label "Northern Territory"^^xsd:string .


###  http://pid.geoscience.org.au/def/ont/link#PlaceNames
:PlaceNames rdf:type owl:NamedIndividual ,
                     :FSDFTheme ;
            rdfs:comment "The Place Names FSDF Theme"@en ;
            rdfs:label "Place Names"^^xsd:string .


###  http://pid.geoscience.org.au/def/ont/link#Positioning
:Positioning rdf:type owl:NamedIndividual ,
                      :FSDFTheme ;
             rdfs:comment "The Positioning FSDF Theme"@en ;
             rdfs:label "Positioning"^^xsd:string .


###  http://pid.geoscience.org.au/def/ont/link#QLD
:QLD rdf:type owl:NamedIndividual ,
              :Jurisdiction ;
     rdfs:comment "The Queensland state government"@en ;
     rdfs:label "Queensland"^^xsd:string .


###  http://pid.geoscience.org.au/def/ont/link#SA
:SA rdf:type owl:NamedIndividual ,
             :Jurisdiction ;
    rdfs:comment "The South Australian state government"@en ;
    rdfs:label "South Australia"^^xsd:string .


###  http://pid.geoscience.org.au/def/ont/link#Transport
:Transport rdf:type owl:NamedIndividual ,
                    :FSDFTheme ;
           rdfs:comment "The Transport FSDF Theme"@en ;
           rdfs:label "Transport"^^xsd:string .


###  http://pid.geoscience.org.au/def/ont/link#VIC
:VIC rdf:type owl:NamedIndividual ,
              :Jurisdiction ;
     rdfs:comment "The Victorian state government"@en ;
     rdfs:label "Victoria"^^xsd:string .


###  http://pid.geoscience.org.au/def/ont/link#WA
:WA rdf:type owl:NamedIndividual ,
             :Jurisdiction ;
    rdfs:comment "The Western Australian state government"@en ;
    rdfs:label "Western Australia"^^xsd:string .


###  http://pid.geoscience.org.au/def/ont/link#Water
:Water rdf:type owl:NamedIndividual ,
                :FSDFTheme ;
       rdfs:comment "The Water FSDF Theme"@en ;
       rdfs:label "Water"^^xsd:string .


###  Generated by the OWL API (version 4.2.8.20170104-2310) https://github.com/owlcs/owlapi
